first commit

Source/Concurrency/LinearDomainCollector.cs
@@ -1,5 +1,5 @@
 using System.Collections.Generic;
-using System.Linq;
+using System.Diagnostics;
 
 namespace Microsoft.Boogie
 {
@@ -13,8 +13,7 @@ namespace Microsoft.Boogie
 
   public class LinearDomain
   {
-    private string domainName;
-    public string DomainName => domainName?? permissionType.ToString();
+    public string DomainName => permissionType.ToString();
     public Type permissionType;
     public Dictionary<Type, Function> collectors;
     public MapType mapTypeBool;
@@ -28,11 +27,10 @@ namespace Microsoft.Boogie
     public Function mapIteInt;
     public Function mapLe;
 
-    public LinearDomain(Program program, string domainName, Type permissionType, Dictionary<Type, Function> collectors)
+    public LinearDomain(Program program, Type permissionType)
     {
-      this.domainName = domainName;
       this.permissionType = permissionType;
-      this.collectors = collectors;
+      this.collectors = new Dictionary<Type, Function>();
 
       this.mapTypeBool = new MapType(Token.NoToken, new List<TypeVariable>(), new List<Type> { this.permissionType },
         Type.Bool);
@@ -66,156 +64,36 @@ namespace Microsoft.Boogie
     {
       return Expr.Eq(expr, ExprHelper.FunctionCall(mapConstBool, Expr.True));
     }
+
+    public void RegisterCollector(Function function)
+    {
+      var inType = function.InParams[0].TypedIdent.Type;
+      if (!collectors.ContainsKey(inType))
+      {
+        collectors.Add(inType, function);
+      }
+    }
   }
-  
+
   class LinearDomainCollector : ReadOnlyVisitor
   {
-    private Program program;
-    private CheckingContext checkingContext;
-    private Dictionary<string, LinearDomain> linearDomains;
-    private HashSet<Type> linearTypes;
-    private HashSet<Type> permissionTypes;
-    private HashSet<Type> visitedTypes;
+    private LinearTypeChecker linearTypeChecker;
+    private Program program => linearTypeChecker.program;
+    private Dictionary<Type, LinearDomain> permissionTypeToLinearDomain;
 
-    private LinearDomainCollector(Program program, CheckingContext checkingContext)
+    private LinearDomainCollector(LinearTypeChecker linearTypeChecker)
     {
-      this.program = program;
-      this.checkingContext = checkingContext;
-      this.linearDomains = new Dictionary<string, LinearDomain>();
-      this.linearTypes = new HashSet<Type>();
-      this.permissionTypes = new HashSet<Type>();
-      this.visitedTypes = new HashSet<Type>();
+      this.linearTypeChecker = linearTypeChecker;
+      this.permissionTypeToLinearDomain = new Dictionary<Type, LinearDomain>();
     }
 
-    public static (Dictionary<string, LinearDomain>, Dictionary<Type, LinearDomain>, HashSet<Type>) Collect(Program program, CheckingContext checkingContext)
+    public static Dictionary<Type, LinearDomain> Collect(LinearTypeChecker linearTypeChecker)
     {
-      var collector = new LinearDomainCollector(program, checkingContext);
-      collector.PopulateLinearDomains();
-      collector.VisitProgram(program);
-      return (collector.linearDomains, collector.MakeLinearDomains(), collector.linearTypes);
+      var collector = new LinearDomainCollector(linearTypeChecker);
+      collector.VisitProgram(linearTypeChecker.program);
+      return collector.permissionTypeToLinearDomain;
     }
-
-    public static LinearKind FindLinearKind(Variable v)
-    {
-      if (QKeyValue.FindAttribute(v.Attributes, x => x.Key == CivlAttributes.LINEAR) != null)
-      {
-        return LinearKind.LINEAR;
-      }
-      if (QKeyValue.FindAttribute(v.Attributes, x => x.Key == CivlAttributes.LINEAR_IN) != null)
-      {
-        return LinearKind.LINEAR_IN;
-      }
-      if (QKeyValue.FindAttribute(v.Attributes, x => x.Key == CivlAttributes.LINEAR_OUT) != null)
-      {
-        return LinearKind.LINEAR_OUT;
-      }
-      return LinearKind.ORDINARY;
-    }
-
-    public static string FindDomainName(Variable v)
-    {
-      string domainName = QKeyValue.FindStringAttribute(v.Attributes, CivlAttributes.LINEAR);
-      if (domainName != null)
-      {
-        return domainName;
-      }
-      domainName = QKeyValue.FindStringAttribute(v.Attributes, CivlAttributes.LINEAR_IN);
-      if (domainName != null)
-      {
-        return domainName;
-      }
-      return QKeyValue.FindStringAttribute(v.Attributes, CivlAttributes.LINEAR_OUT);
-    }
-    
-    private bool ContainsPermissionType(Type type)
-    {
-      if (program.monomorphizer == null)
-      {
-        return false;
-      }
-      if (!visitedTypes.Contains(type))
-      {
-        visitedTypes.Add(type);
-        if (type is CtorType ctorType && ctorType.Decl is DatatypeTypeCtorDecl datatypeTypeCtorDecl)
-        {
-          var originalDecl = Monomorphizer.GetOriginalDecl(datatypeTypeCtorDecl);
-          var originalDeclName = originalDecl.Name;
-          if (CivlPrimitives.LinearTypes.Contains(originalDeclName))
-          {
-            permissionTypes.Add(type);
-            linearTypes.Add(type);
-            var innerType = program.monomorphizer.GetTypeInstantiation(datatypeTypeCtorDecl)[0];
-            ContainsPermissionType(innerType);
-          }
-          else
-          {
-            datatypeTypeCtorDecl.Constructors.ForEach(constructor => constructor.InParams.ForEach(v =>
-            {
-              if (ContainsPermissionType(v.TypedIdent.Type))
-              {
-                linearTypes.Add(type);
-              }
-            }));
-          }
-        }
-        if (type is MapType mapType)
-        {
-          mapType.Arguments.ForEach(argType => ContainsPermissionType(argType));
-          ContainsPermissionType(mapType.Result);
-          if (ContainsPermissionType(mapType.Result))
-          {
-            linearTypes.Add(type);
-          }
-        }
-      }
-      return linearTypes.Contains(type);
-    }
-    
-    private Type GetPermissionType(Type type)
-    {
-      var typeCtorDecl = type.AsCtor.Decl;
-      var originalTypeCtorDecl = Monomorphizer.GetOriginalDecl(typeCtorDecl);
-      var actualTypeParams = program.monomorphizer.GetTypeInstantiation(typeCtorDecl);
-      return actualTypeParams[0];
-    }
-    
-    private Dictionary<Type, LinearDomain> MakeLinearDomains()
-    {
-      var permissionTypeToCollectors = new Dictionary<Type, Dictionary<Type, Function>>();
-      foreach (var type in permissionTypes)
-      {
-        var typeCtorDecl = type.AsCtor.Decl;
-        var originalTypeCtorDecl = Monomorphizer.GetOriginalDecl(typeCtorDecl);
-        var actualTypeParams = program.monomorphizer.GetTypeInstantiation(typeCtorDecl);
-        var permissionType = GetPermissionType(type); 
-        if (!permissionTypeToCollectors.ContainsKey(permissionType))
-        {
-          permissionTypeToCollectors.Add(permissionType, new Dictionary<Type, Function>());
-        }
-        if (!permissionTypeToCollectors[permissionType].ContainsKey(type))
-        {
-          if (originalTypeCtorDecl.Name == "Lmap")
-          {
-            var typeParamInstantiationMap = new Dictionary<string, Type> { { "K", actualTypeParams[0] }, { "V", actualTypeParams[1] } };
-            var collector = program.monomorphizer.InstantiateFunction("Lmap_Collector", typeParamInstantiationMap);
-            permissionTypeToCollectors[permissionType].Add(type, collector);
-          }
-          else
-          {
-            var typeParamInstantiationMap = new Dictionary<string, Type> { { "V", actualTypeParams[0] } };
-            var collector =
-                originalTypeCtorDecl.Name == "Lset"
-                  ? program.monomorphizer.InstantiateFunction("Lset_Collector", typeParamInstantiationMap) :
-                  program.monomorphizer.InstantiateFunction("Lval_Collector", typeParamInstantiationMap);
-            permissionTypeToCollectors[permissionType].Add(type, collector);
-          }
-        }
-      }
-      var permissionTypeToLinearDomain =
-        permissionTypeToCollectors.ToDictionary(kv => kv.Key, kv => new LinearDomain(program, null, kv.Key, kv.Value));
-      return permissionTypes.ToDictionary(type => type, type => permissionTypeToLinearDomain[GetPermissionType(type)]);
-    }
-    
+  
     public override Implementation VisitImplementation(Implementation node)
     {
       // Boogie parser strips the attributes from the parameters of the implementation
@@ -245,142 +123,53 @@ namespace Microsoft.Boogie
 
     public override Variable VisitVariable(Variable node)
     {
-      string domainName = FindDomainName(node);
-      var nodeType = node.TypedIdent.Type;
-      var containsPermissionType = ContainsPermissionType(nodeType);
-      if (domainName != null)
+      if (LinearTypeChecker.FindLinearKind(node) != LinearKind.ORDINARY)
       {
-        if (!linearDomains.ContainsKey(domainName))
-        {
-          checkingContext.Error(node, $"Permission type not declared for domain {domainName}");
-        } 
-        else if (containsPermissionType)
-        {
-          checkingContext.Error(node, $"Variable of linear type must not have a domain name");
-        }
-      }
-      if (containsPermissionType)
-      {
-        if (FindLinearKind(node) == LinearKind.ORDINARY)
-        {
-          node.Attributes = new QKeyValue(Token.NoToken, CivlAttributes.LINEAR, new List<object>(), node.Attributes);
-        }
+        RegisterLinearVariable(node);
       }
       return node;
     }
 
-    private void PopulateLinearDomains()
+    private void RegisterLinearVariable(Variable v)
     {
-      var permissionTypes = new Dictionary<string, Type>();
-      foreach (var decl in program.TopLevelDeclarations.Where(decl => decl is TypeCtorDecl || decl is TypeSynonymDecl))
+      var type = v.TypedIdent.Type;
+      var permissionType = linearTypeChecker.GetPermissionType(type);
+      if (permissionType == null)
       {
-        foreach (var domainName in FindDomainNames(decl.Attributes))
-        {
-          if (permissionTypes.ContainsKey(domainName))
-          {
-            checkingContext.Error(decl, $"Duplicate permission type for domain {domainName}");
-          }
-          else if (decl is TypeCtorDecl typeCtorDecl)
-          {
-            if (typeCtorDecl.Arity > 0)
-            {
-              checkingContext.Error(decl, "Permission type must be fully instantiated");
-            }
-            else
-            {
-              permissionTypes[domainName] = new CtorType(Token.NoToken, typeCtorDecl, new List<Type>());
-            }
-          }
-          else
-          {
-            permissionTypes[domainName] =
-              new TypeSynonymAnnotation(Token.NoToken, (TypeSynonymDecl)decl, new List<Type>());
-          }
-        }
+        return;
       }
-
-      var domainNameToCollectors = new Dictionary<string, Dictionary<Type, Function>>();
-      foreach (var (domainName, permissionType) in permissionTypes)
+      var linearDomain = RegisterPermissionType(permissionType);
+      if (type is CtorType ctorType && ctorType.Decl is DatatypeTypeCtorDecl datatypeTypeCtorDecl)
       {
-        domainNameToCollectors[domainName] = new Dictionary<Type, Function>();
+        var originalTypeCtorDecl = Monomorphizer.GetOriginalDecl(datatypeTypeCtorDecl);
+        var typeName = originalTypeCtorDecl.Name;
+        var actualTypeParams = program.monomorphizer.GetTypeInstantiation(datatypeTypeCtorDecl);
+        if (typeName == "Map")
         {
-          domainNameToCollectors[domainName][permissionType] =
-            program.monomorphizer.InstantiateFunction("MapOne",
-              new Dictionary<string, Type>() { { "T", permissionType } });
+          var typeParamInstantiationMap = new Dictionary<string, Type> { { "T", actualTypeParams[0] }, { "U", actualTypeParams[1] } };
+          linearDomain.RegisterCollector(program.monomorphizer.InstantiateFunction("Map_Collector", typeParamInstantiationMap));
         }
+        else if (typeName == "Set")
         {
-          var type = new MapType(Token.NoToken, new List<TypeVariable>(), new List<Type> { permissionType }, Type.Bool);
-          domainNameToCollectors[domainName][type] =
-            program.monomorphizer.InstantiateFunction("Id", new Dictionary<string, Type>() { { "T", type } });
-        }
-      }
-
-      foreach (var node in program.TopLevelDeclarations.OfType<Function>())
-      {
-        string domainName = QKeyValue.FindStringAttribute(node.Attributes, CivlAttributes.LINEAR);
-        if (domainName == null)
-        {
-          continue;
-        }
-
-        if (!domainNameToCollectors.ContainsKey(domainName))
-        {
-          checkingContext.Error(node, "Domain name has not been declared");
-          continue;
-        }
-
-        if (node.InParams.Count == 1 && node.OutParams.Count == 1)
-        {
-          Type inType = node.InParams[0].TypedIdent.Type;
-          if (domainNameToCollectors[domainName].ContainsKey(inType))
-          {
-            checkingContext.Error(node, "A collector for domain for input type is already defined");
-            continue;
-          }
-
-          var outType = node.OutParams[0].TypedIdent.Type;
-          var expectedType = new MapType(Token.NoToken, new List<TypeVariable>(),
-            new List<Type> { permissionTypes[domainName] }, Type.Bool);
-          if (!outType.Equals(expectedType))
-          {
-            checkingContext.Error(node, "Output of a linear domain collector has unexpected type");
-          }
-          else
-          {
-            domainNameToCollectors[domainName].Add(inType, node);
-          }
+          var typeParamInstantiationMap = new Dictionary<string, Type> { { "T", actualTypeParams[0] } };
+          linearDomain.RegisterCollector(program.monomorphizer.InstantiateFunction("Set_Collector", typeParamInstantiationMap));
         }
         else
         {
-          checkingContext.Error(node, "Linear domain collector should have one input and one output parameter");
+          Debug.Assert(typeName == "One");
+          var typeParamInstantiationMap = new Dictionary<string, Type> { { "T", actualTypeParams[0] } };
+          linearDomain.RegisterCollector(program.monomorphizer.InstantiateFunction("One_Collector", typeParamInstantiationMap));
         }
-      }
-
-      foreach (var (domainName, permissionType) in permissionTypes)
-      {
-        linearDomains.Add(domainName,
-          new LinearDomain(program, domainName, permissionType, domainNameToCollectors[domainName]));
       }
     }
 
-    private static List<string> FindDomainNames(QKeyValue kv)
+    private LinearDomain RegisterPermissionType(Type permissionType)
     {
-      List<string> domains = new List<string>();
-      for (; kv != null; kv = kv.Next)
+      if (!permissionTypeToLinearDomain.ContainsKey(permissionType))
       {
-        if (kv.Key != CivlAttributes.LINEAR)
-        {
-          continue;
-        }
-        foreach (var o in kv.Params)
-        {
-          if (o is string s)
-          {
-            domains.Add(s);
-          }
-        }
+        permissionTypeToLinearDomain[permissionType] = new LinearDomain(program, permissionType);
       }
-      return domains;
+      return permissionTypeToLinearDomain[permissionType];
     }
   }
 }
