Source/Core/node.bpl
@@ -1,54 +1,78 @@
-// RUN: %parallel-boogie "%s" > "%t"
-// RUN: %diff "%s.expect" "%t"
-// XFAIL: *
+datatype Node<T> { Node(next: Option (Loc (Node T)), val: T) }
 
-datatype Node<T> { Node(next: RefNode T, val: T) }
-type RefNode T = Ref (Node T);
-
-function Between<T>(f: [RefNode T]Node T, x: RefNode T, y: RefNode T, z: RefNode T): bool;
-function Avoiding<T>(f: [RefNode T]Node T, x: RefNode T, y: RefNode T, z: RefNode T): bool;
-function {:inline} BetweenSet<T>(f:[RefNode T]Node T, x: RefNode T, z: RefNode T): [RefNode T]bool
+function Between<T>(f: [Loc (Node T)]Node T, x: Option (Loc (Node T)), y: Option (Loc (Node T)), z: Option (Loc (Node T))): bool;
+function Avoiding<T>(f: [Loc (Node T)]Node T, x: Option (Loc (Node T)), y: Option (Loc (Node T)), z: Option (Loc (Node T))): bool;
+function {:inline} BetweenSet<T>(f:[Loc (Node T)]Node T, x: Option (Loc (Node T)), z: Option (Loc (Node T))): [Loc (Node T)]bool
 {
-  (lambda y: RefNode T :: Between(f, x, y, z))
+  (lambda y: Loc (Node T) :: Between(f, x, Some(y), z))
 }
 
 // reflexive
-axiom {:ctor "Node"} (forall<T> f: [RefNode T]Node T, x: RefNode T :: Between(f, x, x, x));
+axiom {:ctor "Node"} (forall<T> f: [Loc (Node T)]Node T, x: Option (Loc (Node T)) :: Between(f, x, x, x));
 
 // step
-axiom {:ctor "Node"} (forall<T> f: [RefNode T]Node T, x: RefNode T, y: RefNode T, z: RefNode T, w: RefNode T :: {Between(f, y, z, w), f[x]} Between(f, x, f[x]->next, f[x]->next));
+axiom {:ctor "Node"} (forall<T> f: [Loc (Node T)]Node T, x: Loc (Node T) :: 
+  {f[x]} 
+  Between(f, Some(x), f[x]->next, f[x]->next));
 
 // reach
-axiom {:ctor "Node"} (forall<T> f: [RefNode T]Node T, x: RefNode T, y: RefNode T :: {f[x], Between(f, x, y, y)} Between(f, x, y, y) ==> x == y || Between(f, x, f[x]->next, y));
+axiom {:ctor "Node"} (forall<T> f: [Loc (Node T)]Node T, x: Loc (Node T), y: Option (Loc (Node T)) :: 
+  {f[x], Between(f, Some(x), y, y)} 
+  Between(f, Some(x), y, y) ==> Some(x) == y || Between(f, Some(x), f[x]->next, y));
 
 // cycle
-axiom {:ctor "Node"} (forall<T> f: [RefNode T]Node T, x: RefNode T, y:RefNode T :: {f[x], Between(f, x, y, y)} f[x]->next == x && Between(f, x, y, y) ==> x == y);
+axiom {:ctor "Node"} (forall<T> f: [Loc (Node T)]Node T, x: Loc (Node T), y: Option (Loc (Node T)) :: 
+  {f[x], Between(f, Some(x), y, y)} 
+  f[x]->next == Some(x) && Between(f, Some(x), y, y) ==> Some(x) == y);
 
 // sandwich
-axiom {:ctor "Node"} (forall<T> f: [RefNode T]Node T, x: RefNode T, y: RefNode T :: {Between(f, x, y, x)} Between(f, x, y, x) ==> x == y);
+axiom {:ctor "Node"} (forall<T> f: [Loc (Node T)]Node T, x: Option (Loc (Node T)), y: Option (Loc (Node T)) :: 
+  {Between(f, x, y, x)} 
+  Between(f, x, y, x) ==> x == y);
 
 // order1
-axiom {:ctor "Node"} (forall<T> f: [RefNode T]Node T, x: RefNode T, y: RefNode T, z: RefNode T :: {Between(f, x, y, y), Between(f, x, z, z)} Between(f, x, y, y) && Between(f, x, z, z) ==> Between(f, x, y, z) || Between(f, x, z, y));
+axiom {:ctor "Node"} (forall<T> f: [Loc (Node T)]Node T, x: Option (Loc (Node T)), y: Option (Loc (Node T)), z: Option (Loc (Node T)) :: 
+  {Between(f, x, y, y), Between(f, x, z, z)} 
+  Between(f, x, y, y) && Between(f, x, z, z) ==> Between(f, x, y, z) || Between(f, x, z, y));
 
 // order2
-axiom {:ctor "Node"} (forall<T> f: [RefNode T]Node T, x: RefNode T, y: RefNode T, z: RefNode T :: {Between(f, x, y, z)} Between(f, x, y, z) ==> Between(f, x, y, y) && Between(f, y, z, z));
+axiom {:ctor "Node"} (forall<T> f: [Loc (Node T)]Node T, x: Option (Loc (Node T)), y: Option (Loc (Node T)), z: Option (Loc (Node T)) :: 
+  {Between(f, x, y, z)} 
+  Between(f, x, y, z) ==> Between(f, x, y, y) && Between(f, y, z, z));
 
 // transitive1
-axiom {:ctor "Node"} (forall<T> f: [RefNode T]Node T, x: RefNode T, y: RefNode T, z: RefNode T :: {Between(f, x, y, y), Between(f, y, z, z)} Between(f, x, y, y) && Between(f, y, z, z) ==> Between(f, x, z, z));
+axiom {:ctor "Node"} (forall<T> f: [Loc (Node T)]Node T, x: Option (Loc (Node T)), y: Option (Loc (Node T)), z: Option (Loc (Node T)) :: 
+  {Between(f, x, y, y), Between(f, y, z, z)} 
+  Between(f, x, y, y) && Between(f, y, z, z) ==> Between(f, x, z, z));
 
 // transitive2
-axiom {:ctor "Node"} (forall<T> f: [RefNode T]Node T, x: RefNode T, y: RefNode T, z: RefNode T, w: RefNode T :: {Between(f, x, y, z), Between(f, y, w, z)} Between(f, x, y, z) && Between(f, y, w, z) ==> Between(f, x, y, w) && Between(f, x, w, z));
+axiom {:ctor "Node"} (forall<T> f: [Loc (Node T)]Node T, x: Option (Loc (Node T)), y: Option (Loc (Node T)), z: Option (Loc (Node T)), w: Option (Loc (Node T)) :: 
+  {Between(f, x, y, z), Between(f, y, w, z)} 
+  Between(f, x, y, z) && Between(f, y, w, z) ==> Between(f, x, y, w) && Between(f, x, w, z));
 
 // transitive3
-axiom {:ctor "Node"} (forall<T> f: [RefNode T]Node T, x: RefNode T, y: RefNode T, z: RefNode T, w: RefNode T :: {Between(f, x, y, z), Between(f, x, w, y)} Between(f, x, y, z) && Between(f, x, w, y) ==> Between(f, x, w, z) && Between(f, w, y, z));
+axiom {:ctor "Node"} (forall<T> f: [Loc (Node T)]Node T, x: Option(Loc (Node T)), y: Option (Loc (Node T)), z: Option (Loc (Node T)), w: Option (Loc (Node T)) :: 
+  {Between(f, x, y, z), Between(f, x, w, y)} 
+  Between(f, x, y, z) && Between(f, x, w, y) ==> Between(f, x, w, z) && Between(f, w, y, z));
 
 // This axiom is required to deal with the incompleteness of the trigger for the reflexive axiom.
 // It cannot be proved using the rest of the axioms.
-axiom {:ctor "Node"} (forall<T> f: [RefNode T]Node T, u:RefNode T, x: RefNode T :: {Between(f, u, x, x)} Between(f, u, x, x) ==> Between(f, u, u, x));
+axiom {:ctor "Node"} (forall<T> f: [Loc (Node T)]Node T, u: Option (Loc (Node T)), x: Option (Loc (Node T)) :: 
+  {Between(f, u, x, x)} 
+  Between(f, u, x, x) ==> Between(f, u, u, x));
 
 // relation between Avoiding and Between
-axiom {:ctor "Node"} (forall<T> f: [RefNode T]Node T, x: RefNode T, y: RefNode T, z: RefNode T :: {Avoiding(f, x, y, z)} Avoiding(f, x, y, z) <==> (Between(f, x, y, z) || (Between(f, x, y, y) && !Between(f, x, z, z))));
-axiom {:ctor "Node"} (forall<T> f: [RefNode T]Node T, x: RefNode T, y: RefNode T, z: RefNode T :: {Between(f, x, y, z)} Between(f, x, y, z) <==> (Avoiding(f, x, y, z) && Avoiding(f, x, z, z)));
+axiom {:ctor "Node"} (forall<T> f: [Loc (Node T)]Node T, x: Option (Loc (Node T)), y: Option (Loc (Node T)), z: Option (Loc (Node T)) :: 
+  {Avoiding(f, x, y, z)} 
+  Avoiding(f, x, y, z) <==> Between(f, x, y, z) || (Between(f, x, y, y) && !Between(f, x, z, z)));
+axiom {:ctor "Node"} (forall<T> f: [Loc (Node T)]Node T, x: Option (Loc (Node T)), y: Option (Loc (Node T)), z: Option (Loc (Node T)) :: 
+  {Between(f, x, y, z)} 
+  Between(f, x, y, z) <==> Avoiding(f, x, y, z) && Avoiding(f, x, z, z));
 
 // update
-axiom {:ctor "Node"} (forall<T> f: [RefNode T]Node T, u: RefNode T, v: RefNode T, x: RefNode T, p: RefNode T, q: Node T :: {Avoiding(f[p := q], u, v, x)} Avoiding(f[p := q], u, v, x) <==> ((Avoiding(f, u, v, p) && Avoiding(f, u, v, x)) || (Avoiding(f, u, p, x) && p != x && Avoiding(f, q->next, v, p) && Avoiding(f, q->next, v, x))));
+axiom {:ctor "Node"} (forall<T> f: [Loc (Node T)]Node T, u: Option (Loc (Node T)), v: Option (Loc (Node T)), x: Option (Loc (Node T)), p: Loc (Node T), q: Node T :: 
+  {Avoiding(f[p := q], u, v, x)} 
+  Avoiding(f[p := q], u, v, x) <==>
+    (Avoiding(f, u, v, Some(p)) && Avoiding(f, u, v, x)) || 
+    (Avoiding(f, u, Some(p), x) && Some(p) != x && Avoiding(f, q->next, v, Some(p)) && Avoiding(f, q->next, v, x))
+);
